feat(library): add functor, applicative, and monad laws, and prove them correct for non-meta instances

library/init/category/applicative.lean
@@ -14,11 +14,31 @@ set_option auto_param.check_exists false
 class applicative (f : Type u → Type v) extends functor f :=
 (pure : Π {α : Type u}, α → f α)
 (seq  : Π {α β : Type u}, f (α → β) → f α → f β)
-(map := λ _ _ x y, seq (pure x) y)
+(infixr ` <$> `:100 := map)
+(infixl ` <*> `:60 := seq)
+(map := λ _ _ x y, pure x <*> y)
+-- ` <* `
 (seq_left : Π {α β : Type u}, f α → f β → f α := λ α β a b, seq (map (const β) a) b)
-(seq_right : Π {α β : Type u}, f α → f β → f β := λ α β a b, seq (map (const α id) a) b)
 (seq_left_eq : ∀ {α β : Type u} (a : f α) (b : f β), seq_left a b = seq (map (const β) a) b . control_laws_tac)
+-- ` *> `
+(seq_right : Π {α β : Type u}, f α → f β → f β := λ α β a b, seq (map (const α id) a) b)
 (seq_right_eq : ∀ {α β : Type u} (a : f α) (b : f β), seq_right a b = seq (map (const α id) a) b . control_laws_tac)
+-- applicative laws
+(pure_seq_eq_map : ∀ {α β : Type u} (g : α → β) (x : f α), pure g <*> x = g <$> x) -- . control_laws_tac)
+(map_pure : ∀ {α β : Type u} (g : α → β) (x : α), g <$> pure x = pure (g x))
+(seq_pure : ∀ {α β : Type u} (g : f (α → β)) (x : α),
+  g <*> pure x = (λ g : α → β, g x) <$> g)
+(seq_assoc : ∀ {α β γ : Type u} (x : f α) (g : f (α → β)) (h : f (β → γ)),
+  h <*> (g <*> x) = (@comp α β γ <$> h) <*> g <*> x)
+-- defaulted functor law
+(map_comp := λ α β γ g h x, calc
+  (h ∘ g) <$> x = pure (h ∘ g) <*> x                        : eq.symm $ pure_seq_eq_map _ _
+            ... = (comp h <$> pure g) <*> x                 : eq.rec rfl $ map_pure (comp h) g
+            ... = pure (@comp α β γ h) <*> pure g <*> x     : eq.rec rfl $ eq.symm $ pure_seq_eq_map (comp h) (pure g)
+            ... = (@comp α β γ <$> pure h) <*> pure g <*> x : eq.rec rfl $ map_pure (@comp α β γ) h
+            ... = pure h <*> (pure g <*> x)                 : eq.symm $ seq_assoc _ _ _
+            ... = h <$> (pure g <*> x)                      : pure_seq_eq_map _ _
+            ... = h <$> g <$> x                             : congr_arg _ $ pure_seq_eq_map _ _)
 end
 
 section
@@ -38,7 +58,12 @@ applicative.seq_left
 @[inline] def seq_right : f α → f β → f β :=
 applicative.seq_right
 
-infixl ` <*> `:2 := seq_app
-infixl ` <* `:2  := seq_left
-infixl ` *> `:2  := seq_right
+infixl ` <*> `:60 := seq_app
+infixl ` <* `:60  := seq_left
+infixl ` *> `:60  := seq_right
+
 end
+
+-- applicative "law" derivable from other laws
+theorem applicative.pure_id_seq {α β : Type u} {f : Type u → Type v} [applicative f] (x : f α) : pure id <*> x = x :=
+eq.trans (applicative.pure_seq_eq_map _ _) (functor.id_map _)
