library/init/category/functor.lean
@@ -13,8 +13,13 @@ set_option auto_param.check_exists false
 
 class functor (f : Type u → Type v) : Type (max u+1 v) :=
 (map : Π {α β : Type u}, (α → β) → f α → f β)
+(infixr ` <$> `:100 := map)
+-- ` <$ `
 (map_const : Π {α : Type u} (β : Type u), α → f β → f α := λ α β, map ∘ const β)
 (map_const_eq : ∀ {α β : Type u}, @map_const α β = map ∘ const β . control_laws_tac)
+-- `functor` is indeed a categorical functor
+(id_map : Π {α : Type u} (x : f α), id <$> x = x)
+(map_comp : Π {α β γ : Type u} (g : α → β) (h : β → γ) (x : f α), (h ∘ g) <$> x = h <$> g <$> x)
 end
 
 @[inline] def fmap {f : Type u → Type v} [functor f] {α β : Type u} : (α → β) → f α → f β :=
