library/init/category/monad.lean
@@ -7,6 +7,8 @@ prelude
 import init.category.applicative
 universes u v
 
+open function
+
 class has_bind (m : Type u → Type v) :=
 (bind : Π {α β : Type u}, m α → (α → m β) → m β)
 
@@ -16,16 +18,63 @@ has_bind.bind
 @[inline] def has_bind.and_then {α β : Type u} {m : Type u → Type v} [has_bind m] (x : m α) (y : m β) : m β :=
 do x, y
 
-infixl ` >>= `:2 := bind
-infixl ` >> `:2  := has_bind.and_then
+infixl ` >>= `:55 := bind
+infixl ` >> `:55  := has_bind.and_then
+
+section
+set_option auto_param.check_exists false
 
 class monad (m : Type u → Type v) extends applicative m, has_bind m : Type (max u+1 v) :=
-(map := λ α β f x, bind x $ λ x, pure (f x))
-(seq := λ α β f x, bind f $ λ f, map f x)
+(infixr ` <$> `:100 := map)
+(infixl ` <*> `:60 := seq)
+(infixl ` >>= `:55 := bind)
+(map := λ α β f x, x >>= pure ∘ f)
+(seq := λ α β f x, f >>= (<$> x))
+(bind_pure_comp_eq_map : ∀ {α β : Type u} (f : α → β) (x : m α), x >>= pure ∘ f = f <$> x  . control_laws_tac)
+(bind_map_eq_seq : ∀ {α β : Type u} (f : m (α → β)) (x : m α), f >>= (<$> x) = f <*> x  . control_laws_tac)
+-- monad laws
+(pure_bind : ∀ {α β : Type u} (x : α) (f : α → m β), pure x >>= f = f x)
+(bind_assoc : ∀ {α β γ : Type u} (x : m α) (f : α → m β) (g : β → m γ),
+  x >>= f >>= g = x >>= λ x, f x >>= g)
+-- all applicative laws are derivable from the monad laws + id_map
+(pure_seq_eq_map := λ α β g x, eq.trans (eq.symm $ bind_map_eq_seq _ _) (pure_bind _ _))
+(map_pure := λ α β g x, eq.trans (eq.symm $ bind_pure_comp_eq_map _ _) (pure_bind _ _))
+(seq_pure := λ α β g x, calc
+  g <*> pure x = g >>= (<$> pure x)            : eq.symm $ bind_map_eq_seq _ _
+           ... = g >>= λ g : α → β, pure (g x) : congr_arg _ $ funext $ λ g, map_pure _ _
+           ... = (λ g : α → β, g x) <$> g      : bind_pure_comp_eq_map _ _)
+(seq_assoc := λ α β γ x g h, calc
+  h <*> (g <*> x)
+      = h >>= (<$> g <*> x) : eq.symm $ bind_map_eq_seq _ _
+  ... = h >>= λ h, pure (@comp α β γ h) >>= (<$> g) >>= (<$> x) : congr_arg _ $ funext $ λ h, (calc
+    h <$> (g <*> x)
+        = g <*> x >>= pure ∘ h : eq.symm $ bind_pure_comp_eq_map _ _
+    ... = g >>= (<$> x) >>= pure ∘ h                    : eq.rec rfl $ eq.symm $ bind_map_eq_seq g x
+    ... = g >>= λ g, g <$> x >>= pure ∘ h               : bind_assoc _ _ _
+    ... = g >>= λ g, pure (h ∘ g) >>= (<$> x)        : congr_arg _ $ funext $ λ g, (calc
+      g <$> x >>= pure ∘ h
+          = x >>= pure ∘ g >>= pure ∘ h        : eq.rec rfl $ eq.symm $ bind_pure_comp_eq_map g x
+      ... = x >>= λ x, pure (g x) >>= pure ∘ h : bind_assoc _ _ _
+      ... = x >>= λ x, pure (h (g x)) : congr_arg _ $ funext $ λ x, pure_bind _ _
+      ... = (h ∘ g) <$> x : bind_pure_comp_eq_map _ _
+      ... = pure (h ∘ g) >>= (<$> x) : eq.symm $ pure_bind _ _)
+    ... = g >>= pure ∘ (@comp α β γ h) >>= (<$> x) : eq.symm $ bind_assoc _ _ _
+    ... = @comp α β γ h <$> g >>= (<$> x) : eq.rec rfl $ bind_pure_comp_eq_map (comp h) g
+    ... = pure (@comp α β γ h) >>= (<$> g) >>= (<$> x) : eq.rec rfl $ eq.symm $ pure_bind (@comp α β γ h) (<$> g))
+  ... = h >>= (λ h, pure (@comp α β γ h) >>= (<$> g)) >>= (<$> x) : eq.symm $ bind_assoc _ _ _
+  ... = h >>= pure ∘ @comp α β γ >>= (<$> g) >>= (<$> x) : eq.rec rfl $ eq.symm $ bind_assoc h (pure ∘ @comp α β γ) (<$> g)
+  ... = (@comp α β γ <$> h) >>= (<$> g) >>= (<$> x) : eq.rec rfl $ bind_pure_comp_eq_map (@comp α β γ) h
+  ... = ((@comp α β γ <$> h) >>= (<$> g)) <*> x : bind_map_eq_seq _ _
+  ... = (@comp α β γ <$> h) <*> g <*> x : eq.rec rfl $ bind_map_eq_seq (@comp α β γ <$> h) g)
+end
 
-def return {m : Type u → Type v} [monad m] {α : Type u} : α → m α :=
+@[reducible] def return {m : Type u → Type v} [monad m] {α : Type u} : α → m α :=
 pure
 
 /- Identical to has_bind.and_then, but it is not inlined. -/
 def has_bind.seq {α β : Type u} {m : Type u → Type v} [has_bind m] (x : m α) (y : m β) : m β :=
 do x, y
+
+-- monad "law" derivable from other laws
+theorem monad.bind_pure {α β : Type u} {m : Type u → Type v} [monad m] (x : m α) : x >>= pure = x :=
+eq.trans (monad.bind_pure_comp_eq_map _ _ _) (functor.id_map _)
