library/init/data/option/instances.lean
@@ -5,6 +5,8 @@ Authors: Leonardo de Moura
 -/
 prelude
 import .basic
+import init.meta.tactic
+
 
 universes u v
 
@@ -13,7 +15,10 @@ universes u v
 | (some a) b := b a
 
 instance : monad option :=
-{pure := @some, bind := @option_bind}
+{pure := @some, bind := @option_bind,
+ id_map := λ α x, option.rec rfl (λ x, rfl) x,
+ pure_bind := λ α β x f, rfl,
+ bind_assoc := λ α β γ x f g, option.rec rfl (λ x, rfl) x}
 
 def option_orelse {α : Type u} : option α → option α → option α
 | (some a) o         := some a
@@ -24,42 +29,3 @@ instance : alternative option :=
 { option.monad with
   failure := @none,
   orelse  := @option_orelse }
-
-def option_t (m : Type u → Type v) [monad m] (α : Type u) : Type v :=
-m (option α)
-
-@[inline] def option_t_bind {m : Type u → Type v} [monad m] {α β : Type u} (a : option_t m α) (b : α → option_t m β)
-                               : option_t m β :=
-show m (option β), from
-do o ← a,
-   match o with
-   | none     := return none
-   | (some a) := b a
-   end
-
-@[inline] def option_t_return {m : Type u → Type v} [monad m] {α : Type u} (a : α) : option_t m α :=
-show m (option α), from
-return (some a)
-
-instance {m : Type u → Type v} [monad m] : monad (option_t m) :=
-{pure := @option_t_return m _, bind := @option_t_bind m _}
-
-def option_t_orelse {m : Type u → Type v} [monad m] {α : Type u} (a : option_t m α) (b : option_t m α) : option_t m α :=
-show m (option α), from
-do o ← a,
-   match o with
-   | none     := b
-   | (some v) := return (some v)
-   end
-
-def option_t_fail {m : Type u → Type v} [monad m] {α : Type u} : option_t m α :=
-show m (option α), from
-return none
-
-instance {m : Type u → Type v} [monad m] : alternative (option_t m) :=
-{ option_t.monad with
-  failure := @option_t_fail m _,
-  orelse  := @option_t_orelse m _ }
-
-def option_t.lift {m : Type u → Type v} [monad m] {α : Type u} (a : m α) : option_t m α :=
-(some <$> a : m (option α))
