library/init/data/option_t.lean
@@ -1,0 +1,71 @@
+/-
+Copyright (c) 2017 Microsoft Corporation. All rights reserved.
+Released under Apache 2.0 license as described in the file LICENSE.
+Authors: Leonardo de Moura
+-/
+prelude
+import init.meta.interactive
+
+universes u v
+
+def option_t (m : Type u → Type v) [monad m] (α : Type u) : Type v :=
+m (option α)
+
+@[inline] def option_t_bind {m : Type u → Type v} [monad m] {α β : Type u} (a : option_t m α) (b : α → option_t m β)
+                               : option_t m β :=
+show m (option β), from
+do o ← a,
+   match o with
+   | none     := return none
+   | (some a) := b a
+   end
+
+@[inline] def option_t_return {m : Type u → Type v} [monad m] {α : Type u} (a : α) : option_t m α :=
+show m (option α), from
+return (some a)
+
+instance {m : Type u → Type v} [monad m] : monad (option_t m) :=
+{pure := @option_t_return m _, bind := @option_t_bind m _,
+ id_map := begin
+   intros,
+   dsimp [option_t_bind],
+   assert h : option_t_bind._match_1 option_t_return = @pure m _ (option α),
+   { apply funext, intro s, cases s, apply rfl, apply rfl },
+   { rw h, apply @monad.bind_pure _ (option α) m },
+ end,
+ pure_bind := begin
+   intros,
+   dsimp [option_t_bind, option_t_return],
+   dsimp [return, pure, bind], -- TODO: fix signature of `pure_bind`
+   rw [monad.pure_bind], apply rfl
+ end,
+ bind_assoc := begin
+   intros,
+   dsimp [option_t_bind, option_t_return, bind],
+   rw [monad.bind_assoc],
+   apply congr_arg, apply funext, intro x,
+   cases x,
+   { dsimp [option_t_bind._match_1, return, pure],
+     rw [monad.pure_bind], apply rfl },
+   { apply rfl }
+ end}
+
+def option_t_orelse {m : Type u → Type v} [monad m] {α : Type u} (a : option_t m α) (b : option_t m α) : option_t m α :=
+show m (option α), from
+do o ← a,
+   match o with
+   | none     := b
+   | (some v) := return (some v)
+   end
+
+def option_t_fail {m : Type u → Type v} [monad m] {α : Type u} : option_t m α :=
+show m (option α), from
+return none
+
+instance {m : Type u → Type v} [monad m] : alternative (option_t m) :=
+{ @option_t.monad m _ with
+  failure := @option_t_fail m _,
+  orelse  := @option_t_orelse m _ }
+
+def option_t.lift {m : Type u → Type v} [monad m] {α : Type u} (a : m α) : option_t m α :=
+(some <$> a : m (option α))
