library/init/data/set.lean
@@ -4,7 +4,7 @@ Released under Apache 2.0 license as described in the file LICENSE.
 Authors: Leonardo de Moura
 -/
 prelude
-import init.meta.tactic
+import init.meta.interactive
 
 universes u v
 def set (α : Type u) := α → Prop
@@ -74,6 +74,18 @@ def image (f : α → β) (s : set α) : set β :=
 {b | ∃ a, a ∈ s ∧ f a = b}
 
 instance : functor set :=
-{map := @set.image}
+{map := @set.image,
+ id_map := begin
+   intros _ s, apply funext, intro b,
+   dsimp [image, set_of],
+   exact propext ⟨λ ⟨b', ⟨_, _⟩⟩, ‹b' = b› ▸ ‹s b'›,
+                  λ _, ⟨b, ⟨‹s b›, rfl⟩⟩⟩,
+ end,
+ map_comp := begin
+   intros, apply funext, intro c,
+   dsimp [image, set_of],
+   exact propext ⟨λ ⟨a, ⟨h₁, h₂⟩⟩, ⟨g a, ⟨⟨a, ⟨h₁, rfl⟩⟩, h₂⟩⟩,
+                  λ ⟨b, ⟨⟨a, ⟨h₁, h₂⟩⟩, h₃⟩⟩, ⟨a, ⟨h₁, h₂^.symm ▸ h₃⟩⟩⟩
+ end}
 
 end set
