library/init/meta/exceptional.lean
@@ -51,4 +51,6 @@ end exceptional
 
 meta instance : monad exceptional :=
 {pure := @exceptional.return, bind := @exceptional.bind,
- map_const_eq := undefined, seq_left_eq := undefined, seq_right_eq := undefined}
+ map_const_eq := undefined, seq_left_eq := undefined, seq_right_eq := undefined,
+ id_map := undefined, pure_bind := undefined, bind_assoc := undefined,
+ bind_pure_comp_eq_map := undefined, bind_map_eq_seq := undefined}
