library/init/meta/vm.lean
@@ -4,7 +4,7 @@ Released under Apache 2.0 license as described in the file LICENSE.
 Authors: Leonardo de Moura
 -/
 prelude
-import init.meta.tactic init.data.option.basic
+import init.meta.tactic init.data.option_t
 import init.meta.mk_dec_eq_instance
 
 meta constant vm_obj : Type
@@ -77,7 +77,9 @@ meta constant vm_core.ret {α : Type} : α → vm_core α
 meta constant vm_core.bind {α β : Type} : vm_core α → (α → vm_core β) → vm_core β
 
 meta instance : monad vm_core :=
-{map := @vm_core.map, pure := @vm_core.ret, bind := @vm_core.bind}
+{map := @vm_core.map, pure := @vm_core.ret, bind := @vm_core.bind,
+ id_map := undefined, pure_bind := undefined, bind_assoc := undefined,
+ bind_pure_comp_eq_map := undefined, bind_map_eq_seq := undefined}
 
 @[reducible] meta def vm (α : Type) : Type := option_t vm_core α
 
