library/init/propext.lean
@@ -25,3 +25,19 @@ propext (iff_true_intro h)
 
 lemma eq_false_intro {a : Prop} (h : ¬a) : a = false :=
 propext (iff_false_intro h)
+
+theorem iff.to_eq {a b : Prop} (h : a ↔ b) : a = b :=
+propext h
+
+theorem iff_eq_eq {a b : Prop} : (a ↔ b) = (a = b) :=
+propext (iff.intro
+  (assume h, iff.to_eq h)
+  (assume h, h^.to_iff))
+
+lemma eq_false {a : Prop} : (a = false) = (¬ a) :=
+have (a ↔ false) = (¬ a), from propext (iff_false a),
+eq.subst (@iff_eq_eq a false) this
+
+lemma eq_true {a : Prop} : (a = true) = a :=
+have (a ↔ true) = a, from propext (iff_true a),
+eq.subst (@iff_eq_eq a true) this
